@prefix brick: <https://brickschema.org/schema/Brick#> .
@prefix occ: <https://brickschema.org/schema/Brick/extension/occupancy#> .
@prefix dash: <http://datashapes.org/dash#> .
@prefix sh: <http://www.w3.org/ns/shacl#> .
@prefix owl: <http://www.w3.org/2002/07/owl#> .
@prefix rdf: <http://www.w3.org/1999/02/22-rdf-syntax-ns#> .
@prefix rdfs: <http://www.w3.org/2000/01/rdf-schema#> .
@prefix skos: <http://www.w3.org/2004/02/skos/core#> .
@prefix foaf: <http://xmlns.com/foaf/0.1/> .
@prefix sdo: <http://schema.org/> .
@prefix dcterms: <http://purl.org/dc/terms#> .
@prefix unit: <http://qudt.org/vocab/unit/> .
@prefix xsd: <http://www.w3.org/2001/XMLSchema#> .

# TODO: name? what are the values of these points?
occ:OccupantActionStream  a   owl:Class, sh:NodeShape ;
    sh:property [
        rdfs:comment "Actions can be associated with occupants" ;
        sh:path brick:isPointOf ;
        dash:hasValueWithClass occ:Occupant ;
    ] ;
    sh:property [
        sh:path occ:surveyed ;
        sh:datatype xsd:boolean ;
        sh:minCount 1 ;
    ] ;
    skos:definition "A data source of occupant actions; an instance is related to an occupant and usually also an equipment. The timeseries contains the actions. This ontology does not take any position on the encoding of those actions.";
    rdfs:subClassOf brick:Point ;
    # TODO: "hasEnumeratedValues" for what is in the timeseries stream itself?
.

occ:OccupantAttitudeStream  a   owl:Class, sh:NodeShape ;
    sh:property [
        rdfs:comment "Attitudes can be associated with occupants" ;
        sh:path brick:isPointOf ;
        dash:hasValueWithClass occ:Occupant ;
    ] ;
    sh:property [
        sh:path occ:surveyed ;
        sh:datatype xsd:boolean ;
        sh:minCount 1 ;
    ] ;
    skos:definition "A data source of occupant attitudes";
    rdfs:subClassOf brick:Point ;
.

occ:OccupantDrink a owl:Class, sh:NodeShape ;
    skos:definition "A timeseries of when an occupant takes a drink" ;
    rdfs:subClassOf occ:OccupantActionStream ;
.

occ:OccupantClothingChange a owl:Class, sh:NodeShape ;
    skos:definition "A timeseries of when an occupant changes clothing. Data should store the CLO rating of the clothing donned after the change" ;
    rdfs:subClassOf occ:OccupantActionStream ;
    sh:property [
        sh:path brick:hasUnit ;
        sh:hasValue occ:Clo ;
    ] ;
.

occ:OccupantThermalSensation a owl:Class, sh:NodeShape ;
    skos:definition "A timeseries of an occupant's thermal sensation, defined by ASHRAE Standard 55 seven-point thermal sensation: -3 (cold) to +3 (hot)." ;
    rdfs:subClassOf occ:OccupantAttitudeStream ;
.

occ:OccupantActivityLevel a owl:Class, sh:NodeShape ;
    skos:definition "A timeseries of an occupant's activity level" ;
    rdfs:subClassOf occ:OccupantAttitudeStream ;
.

occ:OccupantMetabolicRate a owl:Class, sh:NodeShape ;
    skos:definition "A timeseries of an occupant's metabolic rate" ;
    rdfs:subClassOf occ:OccupantAttitudeStream ;
    sh:property [
        sh:path brick:hasUnit ;
        sh:hasValue occ:Met ;
        sh:in ( occ:Met unit:W-PER-M2 unit:BTU_IT-PER-HR ) ;
    ] ;
.

occ:OccupantClothingChange a owl:Class, sh:NodeShape ;
    skos:definition "A timeseries of when an occupant changes clothing. Data should store the CLO rating of the clothing donned after the change" ;
    rdfs:subClassOf occ:OccupantActionStream ;
.

occ:WindowActionStream  a   owl:Class, sh:NodeShape ;
    rdfs:subClassOf occ:OccupantActionStream ;
    sh:property [
        rdfs:comment "Action should be associated with a window" ;
        sh:path brick:isPointOf ;
        dash:hasValueWithClass occ:Window ;
    ] ;
.


occ:BlindsActionStream  a   owl:Class, sh:NodeShape ;
    rdfs:subClassOf occ:OccupantActionStream ;
    sh:property [
        rdfs:comment "Action should be associated with a window" ;
        sh:path brick:isPointOf ;
        dash:hasValueWithClass occ:Window ;
    ] ;
.

occ:ComputerActionStream  a   owl:Class, sh:NodeShape ;
    rdfs:subClassOf occ:OccupantActionStream ;
    sh:property [
        rdfs:comment "Action should be associated with a computer" ;
        sh:path brick:isPointOf ;
        dash:hasValueWithClass occ:Computer ;
    ] ;
.

occ:ThermostatActionStream  a   owl:Class, sh:NodeShape ;
    rdfs:subClassOf occ:OccupantActionStream ;
    sh:property [
        rdfs:comment "Action should be associated with a thermostat" ;
        sh:path brick:isPointOf ;
        dash:hasValueWithClass brick:Thermostat ;
    ] ;
.

occ:DoorActionStream  a   owl:Class, sh:NodeShape ;
    rdfs:subClassOf occ:OccupantActionStream ;
    sh:property [
        rdfs:comment "Action should be associated with a door" ;
        sh:path brick:isPointOf ;
        dash:hasValueWithClass occ:Door ;
    ] ;
.

occ:LightingActionStream  a   owl:Class, sh:NodeShape ;
    rdfs:subClassOf occ:OccupantActionStream ;
    sh:property [
        rdfs:comment "Action should be associated with a lighting equipment" ;
        sh:path brick:isPointOf ;
        dash:hasValueWithClass brick:Lighting_Equipment ;
    ] ;
.

occ:CeilingFanActionStream  a   owl:Class, sh:NodeShape ;
    rdfs:subClassOf occ:OccupantActionStream ;
    sh:property [
        rdfs:comment "Action should be associated with a ceiling fan" ;
        sh:path brick:isPointOf ;
        dash:hasValueWithClass occ:Ceiling_Fan ;
    ] ;
.

occ:CeilingFanActionStream  a   owl:Class, sh:NodeShape ;
    rdfs:subClassOf occ:OccupantActionStream ;
    sh:property [
        rdfs:comment "Action should be associated with a ceiling fan" ;
        sh:path brick:isPointOf ;
        dash:hasValueWithClass occ:Ceiling_Fan ;
    ] ;
.

occ:PortableHeaterActionStream  a   owl:Class, sh:NodeShape ;
    rdfs:subClassOf occ:OccupantActionStream ;
    sh:property [
        rdfs:comment "Action should be associated with a portable heater" ;
        sh:path brick:isPointOf ;
        dash:hasValueWithClass occ:Portable_Heater ;
    ] ;
.

occ:PortableFanActionStream  a   owl:Class, sh:NodeShape ;
    rdfs:subClassOf occ:OccupantActionStream ;
    sh:property [
        rdfs:comment "Action should be associated with a portable fan" ;
        sh:path brick:isPointOf ;
        dash:hasValueWithClass occ:Portable_Fan ;
    ] ;
.


# TODO: issues:
# - surveyed values: "did you adjust the thermostat in the morning"? associated w/ a time interval
# - "did you turn off lights" w/n the past 2 years?
# - Treat survey data separately? For surveyed actions, there is no timestamp

# have "WindowActionStream" as subclass; it should be applied to a window (capture in shacl shape)
# occupant action streams can infer their type based on the equip they are attached to

# probably want subclasses of equipment actions

occ:Occupancy_Presence_Sensor  a   owl:Class, sh:NodeShape ;
    rdfs:subClassOf brick:Occupancy_Sensor ;
    skos:definition "Boolean value of whether or not there is someone in the space at a point in time" ;
    sh:property [
        sh:path brick:isPointOf ;
        sh:class brick:Location ;
    ] ;
.

occ:Occupancy_Count_Sensor  a   owl:Class, sh:NodeShape ;
    skos:definition "Count of number of occupants in a location at a point in time" ;
    rdfs:subClassOf brick:Occupancy_Sensor ;
    sh:property [
        sh:path brick:isPointOf ;
        sh:class brick:Location ;
    ] ;
.

occ:Occupant_Location_Sensor    a   owl:Class, sh:NodeShape ;
    rdfs:subClassOf brick:Occupancy_Sensor ;
    skos:definition "Location of an occupant at a point in time" ;
    sh:property [
        sh:path brick:isPointOf ;
        sh:class brick:Occupant ;
    ] ;
.

occ:Connected_Device_Count a owl:Class, sh:NodeShape ;
    rdfs:subClassOf brick:Occupancy_Sensor ;
    skos:definition "The number of devices connected to a WiFi AP" ;
    sh:property [
        sh:path brick:isPointOf ;
        sh:class brick:Wireless_Access_Point ;
    ] ;
.
